Progress integration

proof/absspec/WOTS.ec
@@ -27,6 +27,11 @@ qed.
 
 (* op nbytexor(a b : nbytes) : nbytes = NBytes.insubd (bytexor (NBytes.val a) (NBytes.val b)). *)
 
+(* prefix of big endian byte representation of a 32-bit word *)
+op toByte(x : W32.t, k : int) : W8.t list =
+    rev (mkseq (fun i => nth W8.zero (to_list (W4u8.unpack8 x)) i) k).
+
+
 (******************************************************************************)
 (* Corresponds to prf_sk in security spec *)
 op prf_keygen : nbytes -> nbytes * adrs -> nbytes.
